src/Causal_CRDT.thy
@@ -2,77 +2,15 @@ theory
   Causal_CRDT
 imports
   Network
-  Ordered_List
-  Convergence
 begin
 
-lemma filter_empty:
-  shows "Set.filter p {} = {}"
-by auto
-
-lemma set_filter_Un:
-  shows "Set.filter p (xs \<union> ys) = Set.filter p xs \<union> Set.filter p ys"
-by auto
-
-corollary set_filter_insert:
-  shows "Set.filter p (Set.insert x xs) = (if p x then Set.insert x (Set.filter p xs) else Set.filter p xs)"
-using set_filter_Un by(auto split: split_if)
-
-lemma finite_filter:
-  assumes "finite A"
-  shows   "finite (Set.filter p A)"
-using assms
-  apply(induction rule: finite.induct)
-  apply(auto simp add: filter_empty)
-  apply(simp add: set_filter_insert)
-done
-
-lemma set_filter_pred:
-  assumes "x \<in> Set.filter p xs"
-  shows   "p x"
-using assms by simp
-
-lemma list_filter_pred:
-  assumes "x \<in> set (List.filter p xs)"
-  shows   "p x"
-using assms by simp
-
-lemma set_elem_nth:
-  assumes "x \<in> set xs"
-  shows   "\<exists>m. m < length xs \<and> xs ! m = x"
-using assms
-  apply(induction xs, auto)
-  apply(rule_tac x="m+1" in exI)
-  apply auto
-done
-
-(*
-lemma (in finite_event_structure) hb_consistent_lt_hb:
-  assumes "hb.hb_consistent cs"
-          "i < j" "j < length cs"
-  shows   "hb (cs ! i) (cs ! j) \<or> \<not> hb (cs ! j) (cs ! i)"
-using assms
-  apply(induction rule: hb.hb_consistent.induct)
-  apply force
-  apply(subgoal_tac "j < length xs \<or> j = length xs")
-  apply(erule disjE)
-  apply clarsimp
-  apply(subst (asm) nth_append, simp)+
-  apply clarsimp
-prefer 2
-  apply force
-  apply(clarsimp simp add: hb_def)
-  apply(subst (asm) nth_append, simp)+
-done
-*)
-
-lemma (in finite_event_structure) hb_consistent_technical:
+lemma (in network_with_ops) hb_consistent_technical:
   assumes "\<And>m n. m < length cs \<Longrightarrow> n < m \<Longrightarrow> cs ! n \<sqsubset>\<^sup>i cs ! m"
-  shows   "hb.hb_consistent (ordered_node_operations cs)"
+  shows   "hb.hb_consistent (node_deliver_messages cs)"
 using assms
   apply -
   apply(induction cs rule: rev_induct)
-  apply(unfold ordered_node_operations_def)
+  apply(unfold node_deliver_messages_def)
   apply force
   apply clarsimp
   apply(case_tac aa; clarsimp)
@@ -127,83 +65,11 @@ defer
   apply clarsimp
 done
 
-lemma horror_size2:
-  assumes "m < length cs"
-          "length cs > 0"
-  shows   "\<exists>xs ys. cs = xs@(cs!m)#ys"
-using assms
-apply (induct m arbitrary: cs)
-apply clarsimp
-apply (rule_tac x="[]" in exI)
-apply (rule_tac x="tl cs" in exI)
-apply clarsimp
-apply (case_tac cs)
-apply force
-apply force
-apply clarsimp
-apply (case_tac cs)
-apply clarsimp
-apply clarsimp
-apply (case_tac "list = []")
-apply clarsimp
-apply (erule_tac x=list in meta_allE)
-apply clarsimp
-apply (rule_tac x="a#xs" in exI)
-apply (rule_tac x="ys" in exI)
-apply clarsimp
-done
-
-lemma horror_size3:
-  assumes "m < length cs"
-          "n < m"
-          "length cs > 1"
-  shows   "\<exists>xs ys zs. xs@(cs!n)#ys@(cs!m)#zs=cs"
-using assms
-apply (induct n arbitrary: cs m)
-apply clarsimp
-apply (rule_tac x="[]" in exI)
-apply clarsimp
-apply (insert horror_size2)
-apply (erule_tac x="m-1" in meta_allE)
-apply (erule_tac x="tl cs" in meta_allE)
-apply clarsimp
-apply (subgoal_tac "m - Suc 0 < length cs - Suc 0")
-apply clarsimp
-apply (rule_tac x=xs in exI)
-apply (rule_tac x=ys in exI)
-apply (subgoal_tac "cs ! m = tl cs ! (m - Suc 0)")
-apply clarsimp
-apply (metis gr_implies_not0 length_0_conv list.collapse nth_Cons_0)
-apply (metis One_nat_def Suc_pred length_tl nth_tl)
-using Suc_leI diff_less_mono apply blast
-apply clarsimp
-apply (thin_tac "(\<And>m cs. m < length cs \<Longrightarrow> cs \<noteq> [] \<Longrightarrow> \<exists>xs ys. cs = xs @ cs ! m # ys)")
-apply (case_tac cs)
-apply clarsimp
-apply clarsimp
-apply (case_tac "list = []")
-apply clarsimp
-apply (erule_tac x=list in meta_allE)
-apply (erule_tac x="m-1" in meta_allE)
-apply clarsimp
-apply (subgoal_tac "m - Suc 0 < length list")
-defer
-apply linarith
-apply clarsimp
-apply (subgoal_tac "n < m - Suc 0")
-defer
-apply linarith
-apply clarsimp
-apply (rule_tac x="a#xs" in exI)
-apply clarsimp
-apply force
-done
-
-corollary (in finite_event_structure)
-  shows "hb.hb_consistent (ordered_node_operations (carriers i))"
+corollary (in network_with_ops)
+  shows "hb.hb_consistent (node_deliver_messages (carriers i))"
   apply(subgoal_tac "carriers i = [] \<or> (\<exists>c. carriers i = [c]) \<or> (length (carriers i) \<ge> 2)")
-  apply(erule disjE, clarsimp simp add: ordered_node_operations_def)
-  apply(erule disjE, clarsimp simp add: ordered_node_operations_def)
+  apply(erule disjE, clarsimp simp add: node_deliver_messages_def)
+  apply(erule disjE, clarsimp simp add: node_deliver_messages_def)
   apply(case_tac aa; clarsimp)
 defer
   apply(cases "carriers i"; clarsimp; case_tac "list"; clarsimp)
