src/Util.thy
@@ -1,0 +1,233 @@
+theory
+  Util
+imports
+  Main
+begin
+
+lemma distinct_set_notin:
+  assumes "distinct (x#xs)"
+  shows   "x \<notin> set xs"
+using assms by(induction xs, auto)
+
+lemma set_insert_inject:
+  assumes "a \<notin> set xs"
+          "a \<notin> set ys" 
+          "set (a#xs) = set (a#ys)"
+  shows   "set xs = set ys"
+using assms by (induction xs arbitrary: ys) fastforce+
+
+lemma remove1_head:
+  shows "remove1 x (x#xs) = xs"
+  by(induction xs, auto)
+
+lemma set_membership_equality_technicalD [dest]:
+  assumes "{x} \<union> (set xs) = {y} \<union> (set ys)"
+  shows "x = y \<or> y \<in> set xs"
+using assms by(induction xs, auto)
+
+lemma set_equality_technical:
+  assumes "{x} \<union> (set xs) = {y} \<union> (set ys)"
+          "x \<notin> set xs" "y \<notin> set ys" "y \<in> set xs"
+  shows "{x} \<union> (set xs - {y}) = set ys"
+using assms by (induction xs) auto
+
+lemma fold_comp_eq:
+  shows "fold op \<circ> xs x = fold op \<circ> xs id \<circ> x"
+  apply(induction xs rule: rev_induct)
+  apply auto
+done
+
+lemma prefix_eq_distinct_list: "distinct xs \<Longrightarrow> pre1@ys = xs \<Longrightarrow> pre2@ys = xs \<Longrightarrow> pre1 = pre2"
+  apply (induct xs arbitrary: pre1 pre2)
+  apply clarsimp
+  apply (case_tac pre1)
+  apply (thin_tac "(\<And>pre1 pre2. distinct xs \<Longrightarrow> pre1 @ ys = xs \<Longrightarrow> pre2 @ ys = xs \<Longrightarrow> pre1 = pre2)")
+  apply clarsimp
+  apply (case_tac pre2)
+  apply (thin_tac "(\<And>pre1 pre2. distinct xs \<Longrightarrow> pre1 @ ys = xs \<Longrightarrow> pre2 @ ys = xs \<Longrightarrow> pre1 = pre2)")
+  apply clarsimp
+  apply (erule_tac x=list in meta_allE)
+  apply (erule_tac x=lista in meta_allE)
+  apply clarsimp
+done
+
+lemma list_nill_or_snoc: "xs = [] \<or> (\<exists>y ys. xs = ys@[y])"
+  by (induct xs, auto)
+
+lemma suffix_eq_distinct_list: "distinct xs \<Longrightarrow> ys@suf1 = xs \<Longrightarrow> ys@suf2 = xs \<Longrightarrow> suf1 = suf2"
+  apply (induct xs  arbitrary: suf1 suf2 rule: rev_induct)
+  apply clarsimp
+  apply clarsimp
+  apply (subgoal_tac "suf1 = [] \<or> (\<exists>y ys. suf1 = ys@[y])")
+  apply (subgoal_tac "suf2 = [] \<or> (\<exists>y ys. suf2 = ys@[y])")
+  apply (erule disjE, clarsimp)
+  apply clarsimp
+  using list_nill_or_snoc apply auto
+done
+
+lemma pre_suf_eq_distinct_list: "distinct xs \<Longrightarrow> ys \<noteq> [] \<Longrightarrow> pre1@ys@suf1 = xs \<Longrightarrow> pre2@ys@suf2 = xs \<Longrightarrow> pre1 = pre2 \<and> suf1 = suf2"
+  apply (induct xs arbitrary: pre1 pre2 ys)
+  apply clarsimp
+  apply (case_tac pre1)
+  apply (thin_tac " (\<And>pre1 pre2 ys. distinct xs \<Longrightarrow> ys \<noteq> [] \<Longrightarrow> pre1 @ ys @ suf1 = xs \<Longrightarrow> pre2 @ ys @ suf2 = xs \<Longrightarrow> pre1 = pre2 \<and> suf1 = suf2)")
+  apply clarsimp
+  apply (case_tac pre2)
+  apply clarsimp
+  apply (rule_tac xs="a#xs" in suffix_eq_distinct_list)
+  apply force
+  apply assumption
+  apply assumption
+  apply clarsimp
+  apply (metis append_eq_Cons_conv list.set_intros(1))
+  apply (case_tac pre2)
+  apply (thin_tac " (\<And>pre1 pre2 ys. distinct xs \<Longrightarrow> ys \<noteq> [] \<Longrightarrow> pre1 @ ys @ suf1 = xs \<Longrightarrow> pre2 @ ys @ suf2 = xs \<Longrightarrow> pre1 = pre2 \<and> suf1 = suf2)")
+  apply clarsimp
+  apply (metis append_eq_Cons_conv list.set_intros(1))
+  apply (erule_tac x=list in meta_allE, erule_tac x=lista in meta_allE, erule_tac x=ys in meta_allE)
+  apply clarsimp
+done
+
+fun merge :: "('a \<Rightarrow> 'a \<Rightarrow> bool) \<Rightarrow> 'a list \<Rightarrow> 'a list \<Rightarrow> 'a list" where
+  "merge cmp []     ys     = ys" |
+  "merge cmp xs     []     = xs" |
+  "merge cmp (x#xs) (y#ys) =
+     (if cmp x y then
+        x#merge cmp xs (y#ys)
+      else
+        y#merge cmp (x#xs) ys)"
+
+function (sequential) qsort :: "('a \<Rightarrow> 'a \<Rightarrow> bool) \<Rightarrow> 'a list \<Rightarrow> 'a list" where
+  "qsort cmp []      = []" |
+  "qsort cmp [x]     = [x]" |
+  "qsort cmp (x#xs)  =
+     (let ls = List.filter (\<lambda>y. cmp x y) xs;
+          rs = List.filter (\<lambda>y. cmp y x) xs
+      in (qsort cmp ls) @ [x] @ (qsort cmp rs))"
+by pat_completeness auto
+
+termination qsort
+  apply(relation "measure (\<lambda>(cmp, xs). size xs)")
+  apply auto
+  apply(simp_all add: le_imp_less_Suc)
+  using le_imp_less_Suc less_Suc_eq apply auto
+done
+
+lemma qsort_set_mem_preserve:
+  shows "(\<forall>x \<in> set xs. \<forall>y \<in> set xs. cmp x y \<or> cmp y x) \<longrightarrow> set xs = set (qsort cmp xs)"
+  apply(induction rule: qsort.induct[where P="\<lambda>cmp xs. (\<forall>x \<in> set xs. \<forall>y \<in> set xs. cmp x y \<or> cmp y x) \<longrightarrow> set xs = set (qsort cmp xs)"])
+  apply auto
+done
+
+lemma filter_empty:
+  shows "Set.filter p {} = {}"
+by auto
+
+lemma set_filter_Un:
+  shows "Set.filter p (xs \<union> ys) = Set.filter p xs \<union> Set.filter p ys"
+by auto
+
+corollary set_filter_insert:
+  shows "Set.filter p (Set.insert x xs) = (if p x then Set.insert x (Set.filter p xs) else Set.filter p xs)"
+using set_filter_Un by(auto split: split_if)
+
+lemma finite_filter:
+  assumes "finite A"
+  shows   "finite (Set.filter p A)"
+using assms
+  apply(induction rule: finite.induct)
+  apply(auto simp add: filter_empty)
+  apply(simp add: set_filter_insert)
+done
+
+lemma set_filter_pred:
+  assumes "x \<in> Set.filter p xs"
+  shows   "p x"
+using assms by simp
+
+lemma list_filter_pred:
+  assumes "x \<in> set (List.filter p xs)"
+  shows   "p x"
+using assms by simp
+
+lemma set_elem_nth:
+  assumes "x \<in> set xs"
+  shows   "\<exists>m. m < length xs \<and> xs ! m = x"
+using assms
+  apply(induction xs, auto)
+  apply(rule_tac x="m+1" in exI)
+  apply auto
+done
+
+lemma horror_size2:
+  assumes "m < length cs"
+          "length cs > 0"
+  shows   "\<exists>xs ys. cs = xs@(cs!m)#ys"
+using assms
+apply (induct m arbitrary: cs)
+apply clarsimp
+apply (rule_tac x="[]" in exI)
+apply (rule_tac x="tl cs" in exI)
+apply clarsimp
+apply (case_tac cs)
+apply force
+apply force
+apply clarsimp
+apply (case_tac cs)
+apply clarsimp
+apply clarsimp
+apply (case_tac "list = []")
+apply clarsimp
+apply (erule_tac x=list in meta_allE)
+apply clarsimp
+apply (rule_tac x="a#xs" in exI)
+apply (rule_tac x="ys" in exI)
+apply clarsimp
+done
+
+lemma horror_size3:
+  assumes "m < length cs"
+          "n < m"
+          "length cs > 1"
+  shows   "\<exists>xs ys zs. xs@(cs!n)#ys@(cs!m)#zs=cs"
+using assms
+apply (induct n arbitrary: cs m)
+apply clarsimp
+apply (rule_tac x="[]" in exI)
+apply clarsimp
+apply (insert horror_size2)
+apply (erule_tac x="m-1" in meta_allE)
+apply (erule_tac x="tl cs" in meta_allE)
+apply clarsimp
+apply (subgoal_tac "m - Suc 0 < length cs - Suc 0")
+apply clarsimp
+apply (rule_tac x=xs in exI)
+apply (rule_tac x=ys in exI)
+apply (subgoal_tac "cs ! m = tl cs ! (m - Suc 0)")
+apply clarsimp
+apply (metis gr_implies_not0 length_0_conv list.collapse nth_Cons_0)
+apply (metis One_nat_def Suc_pred length_tl nth_tl)
+using Suc_leI diff_less_mono apply blast
+apply clarsimp
+apply (thin_tac "(\<And>m cs. m < length cs \<Longrightarrow> cs \<noteq> [] \<Longrightarrow> \<exists>xs ys. cs = xs @ cs ! m # ys)")
+apply (case_tac cs)
+apply clarsimp
+apply clarsimp
+apply (case_tac "list = []")
+apply clarsimp
+apply (erule_tac x=list in meta_allE)
+apply (erule_tac x="m-1" in meta_allE)
+apply clarsimp
+apply (subgoal_tac "m - Suc 0 < length list")
+defer
+apply linarith
+apply clarsimp
+apply (subgoal_tac "n < m - Suc 0")
+defer
+apply linarith
+apply clarsimp
+apply (rule_tac x="a#xs" in exI)
+apply clarsimp
+apply force
+done
+
+end
